src/Examples/MailServer/MailRefinement.v
@@ -50,7 +50,15 @@ Definition init_base `{@GoModelWf gm} (s: GoLayer.Go.State) :=
 
 Definition init_absr `{@GoModelWf gm} sa sc := Mail.initP sa ∧ init_base sc.
 
-Lemma mail_crash_refinement_seq `{@GoModelWf gm} {T} σ1c σ1a esa esc:
+Definition myΣ {gm} {Hgwf: GoModelWf gm} : gFunctors :=
+  #[@gooseΣ gm Hgwf; @cfgΣ Mail.Op Mail.l;
+    ghost_mapΣ ghost_init_statusC; ghost_mapΣ contentsC;
+    gen_heapΣ string (Filesys.FS.Inode)].
+
+Existing Instance subG_goosePreG.
+Existing Instance subG_cfgPreG.
+
+Lemma mail_crash_refinement_seq {gm} {Hgmwf: @GoModelWf gm} {T} σ1c σ1a esa esc:
   init_absr σ1a σ1c →
   wf_client_seq esa →
   compile_rel_proc_seq mail_impl esa esc →
@@ -59,4 +67,108 @@ Lemma mail_crash_refinement_seq `{@GoModelWf gm} {T} σ1c σ1a esa esc:
                                       (rec_singleton MailServer.Recover) (1, σ1c) (Val σ2c res) →
   ∃ σ2a, proc_exec_seq Mail.l esa (rec_singleton (Ret tt)) (1, σ1a) (Val σ2a res).
 Proof.
+  eapply (@exmach_crash_refinement_seq gm Hgmwf (@myΣ gm Hgmwf)) with
+      (Λa := Mail.l)
+      (es := esa)
+      (T := T)
+      (exec_inv := fun H1 H2 => (∃ hGTmp, @ExecInv gm Hgmwf myΣ H2 H1 _ _ hGTmp)%I)
+      (exec_inner := fun H1 H2 => True%I)
+      (crash_inner := fun H1 H2 => True%I)
+      (*
+      (crash_inner := fun H1 H2 => (@CrashInner myΣ H2 H1)%I)
+       *)
+      (crash_param := fun H1 H2 => unit)
+      (crash_inv := fun H1 H2 _ => @CrashInv _ _ myΣ H2 H1 _ _)
+      (crash_starter := fun H1 H2 _ => @CrashStarter _ _ myΣ H2)
+      (E := nclose sourceN).
+  { apply _. }
+  { apply _. }
+  { intros. apply _. }
+  { intros. apply _. }
+  { set_solver+. }
+  {
+    intros ???? j K Hctx p p' Hcompile. iIntros "(Hj&Hreg&Hexec)".
+    iDestruct "Hexec" as (hGTmp) "Hexec". inversion Hcompile; inj_pair2.
+    - iApply (open_refinement with "[$]"). iIntros "!>".
+      iIntros (?) "(?&?)"; iFrame.
+    - iApply (pickup_refinement with "[$]"). iIntros "!>".
+      iIntros (?) "(?&?)"; iFrame.
+    - iApply (deliver_refinement with "[$]"). iIntros "!>".
+      iIntros (?) "(?&?)"; iFrame.
+    - iApply (delete_refinement with "[$]"). iIntros "!>".
+      iIntros (?) "(?&?)"; iFrame.
+    - iApply (unlock_refinement with "[$]"). iIntros "!>".
+      iIntros (?) "(?&?)"; iFrame.
+    - admit. (* data op refinement, which is partial so far *)
+  }
+  { intros. iIntros "H". iDestruct "H" as (hGTmp ??) "($&?)". }
+  { intros. iIntros "(Hrest&Hreg&Hstarter)".
+    iDestruct "Hrest" as (Γ γ) "(#Hsource&#Hinv)".
+    iDestruct "Hstarter" as (tmps) "(Htmps&Hlock)".
+    wp_bind. wp_bind.
+    iApply (wp_list_start with "[$]").
+    iIntros "!> Hlock".
+    iApply (wp_list_finish with "[$]").
+    iIntros (s ltmps) "!> (Hltmps&Hs&Htmps&Hlock)".
+    iDestruct "Hltmps" as %Hltmps.
+    iAssert (SpoolDir ↦{-1} (tmps ∖ list_to_set (take 0 ltmps)))%I with "[Htmps]" as "Htmps".
+    { by rewrite difference_empty_L. }
+    iDestruct (slice_mapsto_len with "Hs") as %->.
+    assert (0 <= length ltmps) as Hlen by lia.
+    revert Hlen.
+    remember 0 as i eqn:Heq_i.
+    intros Hlen.
+    rewrite [a in S a]Heq_i.
+    clear Heq_i.
+    iLöb as "IH" forall (i Hlen).
+    wp_loop.
+    destruct equal as [Heqlen|Hneq].
+    - subst.
+      rewrite firstn_all.
+      (* in a sense we do not even need to argue that the spool dir is actually empty at
+         this point, it is totally irrelevant *)
+      wp_ret. wp_ret. iNext.
+      iInv "Hinv" as "H" "_".
+      iDestruct "H" as (σ) "(>Hstate&Hmsgs&>Hheap&>Htmp)".
+      iApply (fupd_mask_weaken _ _).
+      { solve_ndisj. }
+      iExists _, _.
+      iFrame. iSplitL "".
+      { iPureIntro. do 2 eexists; split; econstructor. }
+      iClear "Hsource".
+      iIntros (???) "(#Hsource&Hstate)".
+      (* todo: prove execinner for new run *)
+      admit.
+    - wp_bind.
+      destruct (nth_error ltmps i) as [curr_name|] eqn:Heq_curr_name; last first.
+      { exfalso. eapply nth_error_Some; eauto.  inversion Hlen; try congruence; try lia. }
+      iApply (wp_sliceRead with "[$]"); first eauto.
+      iIntros "!> Hs".
+      wp_bind.
+      iInv "Hinv" as "H".
+      iDestruct "H" as (σ) "(>Hstate&Hmsgs&>Hheap&>Htmp)".
+      iDestruct "Htmp" as (tmps_map) "(Hdir&Hpaths)".
+      iDestruct (mapsto_agree with "[$] [$]") as %Heq_dom.
+      rewrite Heq_dom.
+      iDestruct (read_split_join with "[Htmps Hdir]") as "Hdir".
+      { iFrame. replace 1%Z with (S O : Z) by auto. iFrame. }
+      assert (curr_name ∈ tmps ∖ list_to_set (take i ltmps)).
+      { admit. }
+      assert (∃ v, tmps_map !! curr_name = Some v) as (inode&Hcurr_inode).
+      { admit. }
+      iDestruct (big_sepM_delete with "Hpaths") as "(Hcurr&Hpaths)"; eauto.
+      iApply (wp_delete with "[$]").
+      iIntros "!> (Hdir&Hdirlock)".
+      iExists _. iFrame.
+      iDestruct (read_split_join _ 0 with "Hdir") as "(Hdir&Htmps)".
+      iSplitL "Hdir Hpaths".
+      { iModIntro. iNext. iExists _. iFrame.
+        rewrite dom_delete_L. rewrite Heq_dom. iFrame. }
+      wp_ret. iModIntro. iNext.
+      iApply ("IH" with "[] [$] [$] [$] [Htmps]").
+      { iPureIntro. inversion Hlen; try congruence; try lia. }
+      rewrite difference_difference_L.
+      (* todo: prove list_to_set (take (i+1 ltmps) gives you union of take i ltmps with curr *)
+      admit.
+  }
 Abort.
